src/Dmajor.v
@@ -8,7 +8,10 @@ Require Import compcert.common.Globalenvs.
 Require Import compcert.common.Memory.
 Require Import compcert.common.Events.
 Require Import compcert.common.Switch.
-Require Import compcert.common.Smallstep.
+(*Require Import compcert.common.Smallstep.*)
+
+Require Import TraceSemantics.
+Require Import HighValues.
 
 Require Import List.
 Import ListNotations.
@@ -249,6 +252,7 @@ Inductive step: state -> trace -> state -> Prop :=
       step (Returnstate v (Kcall optid f e k) m)
         E0 (State f Sskip k (set_optvar optid v e) m).
 
+
 End RELSEM.
 
 
@@ -262,15 +266,16 @@ Inductive initial_state (p: program): state -> Prop :=
       initial_state p (Callstate f nil Kstop m0).
 
 (** A final state is a [Returnstate] with an empty continuation. *)
+Inductive final_state (p : program): state -> value -> Prop :=
+| final_state_intro: forall v m v',
+    value_inject (Genv.globalenv p) m v v' ->
+    final_state p (Returnstate v' Kstop m) v.
 
-Inductive final_state: state -> int -> Prop :=
-  | final_state_intro: forall r m,
-      final_state (Returnstate (Vint r) Kstop m) r.
 
 (** The corresponding small-step semantics. *)
 
 Definition semantics (p: program) :=
-  Semantics step (initial_state p) final_state (Genv.globalenv p).
+  Semantics step (initial_state p) (final_state p) (Genv.globalenv p).
 
 (** This semantics is receptive to changes in events. *)
 
