src/OeufCompcertCompiler.v
@@ -1,0 +1,160 @@
+(** Libraries. *)
+Require Import String.
+Require Import compcert.lib.Coqlib.
+Require Import compcert.common.Errors.
+Require Import compcert.common.AST.
+Require Import TraceSemantics.
+(** Languages (syntax and semantics). *)
+Require compcert.backend.Cminor.
+Require compcert.backend.CminorSel.
+Require compcert.backend.RTL.
+Require compcert.backend.LTL.
+Require compcert.backend.Linear.
+Require compcert.backend.Mach.
+Require compcert.ia32.Asm.
+(** Translation passes. *)
+Require compcert.backend.Selection.
+Require compcert.backend.RTLgen.
+Require compcert.backend.Tailcall.
+Require compcert.backend.Inlining.
+Require compcert.backend.Renumber.
+Require compcert.backend.Constprop.
+Require compcert.backend.CSE.
+Require compcert.backend.Deadcode.
+Require compcert.backend.Unusedglob.
+Require compcert.backend.Allocation.
+Require compcert.backend.Tunneling.
+Require compcert.backend.Linearize.
+Require compcert.backend.CleanupLabels.
+Require compcert.backend.Debugvar.
+Require compcert.backend.Stacking.
+Require compcert.ia32.Asmgen.
+
+
+
+(** Pretty-printers (defined in Caml). *)
+Parameter print_Cminor: Cminor.program -> unit.
+Parameter print_RTL: Z -> RTL.program -> unit.
+Parameter print_LTL: LTL.program -> unit.
+Parameter print_Mach: Mach.program -> unit.
+
+
+Open Local Scope string_scope.
+
+(** * Composing the translation passes *)
+
+(** We first define useful monadic composition operators,
+    along with funny (but convenient) notations. *)
+
+Definition apply_total (A B: Type) (x: res A) (f: A -> B) : res B :=
+  match x with Error msg => Error msg | OK x1 => OK (f x1) end.
+
+Definition apply_partial (A B: Type)
+                         (x: res A) (f: A -> res B) : res B :=
+  match x with Error msg => Error msg | OK x1 => f x1 end.
+
+Notation "a @@@ b" :=
+   (apply_partial _ _ a b) (at level 50, left associativity).
+Notation "a @@ b" :=
+   (apply_total _ _ a b) (at level 50, left associativity).
+
+Definition print {A: Type} (printer: A -> unit) (prog: A) : A :=
+  let unused := printer prog in prog.
+
+Definition time {A B: Type} (name: string) (f: A -> B) : A -> B := f.
+
+Definition total_if {A: Type}
+          (flag: unit -> bool) (f: A -> A) (prog: A) : A :=
+  if flag tt then f prog else prog.
+
+Definition partial_if {A: Type}
+          (flag: unit -> bool) (f: A -> res A) (prog: A) : res A :=
+  if flag tt then f prog else OK prog.
+
+(** We define three translation functions for whole programs: one
+  starting with a C program, one with a Cminor program, one with an
+  RTL program.  The three translations produce Asm programs ready for
+  pretty-printing and assembling. *)
+
+
+Definition transf_rtl_program (f: RTL.program) : res Asm.program :=
+   OK f
+   @@ print (print_RTL 0)
+   @@ total_if Compopts.optim_tailcalls (time "Tail calls" Tailcall.transf_program)
+   @@ print (print_RTL 1)
+  @@@ time "Inlining" Inlining.transf_program
+   @@ print (print_RTL 2)
+   @@ time "Renumbering" Renumber.transf_program
+   @@ print (print_RTL 3)
+   @@ total_if Compopts.optim_constprop (time "Constant propagation" Constprop.transf_program)
+   @@ print (print_RTL 4)
+   @@ total_if Compopts.optim_constprop (time "Renumbering" Renumber.transf_program)
+   @@ print (print_RTL 5)
+  @@@ partial_if Compopts.optim_CSE (time "CSE" CSE.transf_program)
+   @@ print (print_RTL 6)
+  @@@ partial_if Compopts.optim_redundancy (time "Redundancy elimination" Deadcode.transf_program)
+   @@ print (print_RTL 7)
+  @@@ time "Unused globals" Unusedglob.transform_program
+   @@ print (print_RTL 8)
+  @@@ time "Register allocation" Allocation.transf_program
+   @@ print print_LTL
+   @@ time "Branch tunneling" Tunneling.tunnel_program
+  @@@ time "CFG linearization" Linearize.transf_program
+   @@ time "Label cleanup" CleanupLabels.transf_program
+  @@@ partial_if Compopts.debug (time "Debugging info for local variables" Debugvar.transf_program)
+  @@@ time "Mach generation" Stacking.transf_program
+   @@ print print_Mach
+  @@@ time "Asm generation" Asmgen.transf_program.
+
+Definition transf_cminor_program (p: Cminor.program) : res Asm.program :=
+   OK p
+   @@ print print_Cminor
+  @@@ time "Instruction selection" Selection.sel_program
+  @@@ time "RTL generation" RTLgen.transl_program
+  @@@ transf_rtl_program.
+
+
+Lemma print_identity:
+  forall (A: Type) (printer: A -> unit) (prog: A),
+  print printer prog = prog.
+Proof.
+  intros; unfold print. destruct (printer prog); auto.
+Qed.
+
+Lemma compose_print_identity:
+  forall (A: Type) (x: res A) (f: A -> unit),
+  x @@ print f = x.
+Proof.
+  intros. destruct x; simpl. rewrite print_identity. auto. auto.
+Qed.
+
+Remark forward_simulation_identity:
+  forall sem, forward_simulation sem sem.
+Proof.
+  intros. apply forward_simulation_step with (fun s1 s2 => s2 = s1); intros.
+- exists s1; auto.
+- subst s2; auto.
+- subst s2. exists s1'; auto.
+Qed.
+
+Lemma total_if_simulation:
+  forall (A: Type) (sem: A -> semantics) (flag: unit -> bool) (f: A -> A) (prog: A),
+  (forall p, forward_simulation (sem p) (sem (f p))) ->
+  forward_simulation (sem prog) (sem (total_if flag f prog)).
+Proof.
+  intros. unfold total_if. destruct (flag tt). auto. apply forward_simulation_identity.
+Qed.
+
+Lemma partial_if_simulation:
+  forall (A: Type) (sem: A -> semantics) (flag: unit -> bool) (f: A -> res A) (prog tprog: A),
+  partial_if flag f prog = OK tprog ->
+  (forall p tp, f p = OK tp -> forward_simulation (sem p) (sem tp)) ->
+  forward_simulation (sem prog) (sem tprog).
+Proof.
+  intros. unfold partial_if in *. destruct (flag tt). eauto. inv H. apply forward_simulation_identity.
+Qed.
+
+Theorem transf_rtl_program_correct:
+  forall p tp,
+  transf_rtl_program p = OK tp ->
+  forward_simulation (RTL.semantics p) (Asm.semantics tp).
