src/OeufCompcertSimulations.v
@@ -1,0 +1,118 @@
+(** Libraries. *)
+Require Import String.
+Require Import compcert.lib.Coqlib.
+Require Import compcert.common.Errors.
+Require Import compcert.common.AST.
+Require Import TraceSemantics.
+(** Languages (syntax and semantics). *)
+Require compcert.backend.Cminor.
+Require compcert.backend.CminorSel.
+Require compcert.backend.RTL.
+Require compcert.backend.LTL.
+Require compcert.backend.Linear.
+Require compcert.backend.Mach.
+Require compcert.ia32.Asm.
+(** Translation passes. *)
+Require compcert.backend.Selection.
+Require compcert.backend.RTLgen.
+Require compcert.backend.Tailcall.
+Require compcert.backend.Inlining.
+Require compcert.backend.Renumber.
+Require compcert.backend.Constprop.
+Require compcert.backend.CSE.
+Require compcert.backend.Deadcode.
+Require compcert.backend.Unusedglob.
+Require compcert.backend.Allocation.
+Require compcert.backend.Tunneling.
+Require compcert.backend.Linearize.
+Require compcert.backend.CleanupLabels.
+Require compcert.backend.Debugvar.
+Require compcert.backend.Stacking.
+Require compcert.ia32.Asmgen.
+(** Proofs of semantic preservation. *)
+Require compcert.backend.Selectionproof.
+Require compcert.backend.RTLgenproof.
+Require compcert.backend.Tailcallproof.
+Require compcert.backend.Inliningproof.
+Require compcert.backend.Renumberproof.
+Require compcert.backend.Constpropproof.
+Require compcert.backend.CSEproof.
+Require compcert.backend.Deadcodeproof.
+Require compcert.backend.Unusedglobproof.
+Require compcert.backend.Allocproof.
+Require compcert.backend.Tunnelingproof.
+Require compcert.backend.Linearizeproof.
+Require compcert.backend.CleanupLabelsproof.
+Require compcert.backend.Debugvarproof.
+Require compcert.backend.Stackingproof.
+Require compcert.ia32.Asmgenproof.
+
+Require Import HighValues.
+Require Import compcert.common.Globalenvs.
+
+Require Import StructTact.StructTactics.
+Require Import StructTact.Util.
+
+Require Import EricTact.
+
+(* Cminor bridge *)
+Require Import Cmajor.
+  
+Inductive cminorsel_final_state(p : CminorSel.program): CminorSel.state -> value -> Prop :=
+| cminorsel_final_state_intro: forall v v' m,
+    value_inject (Genv.globalenv p) m v v' ->
+    cminorsel_final_state p (CminorSel.Returnstate v' CminorSel.Kstop m) v.
+
+Definition CminorSel_semantics (p: CminorSel.program) :=
+  Semantics CminorSel.step (CminorSel.initial_state p) (cminorsel_final_state p) (Genv.globalenv p).
+
+
+Lemma cminorsel_final_states :
+  forall prog tprog,
+    Selection.sel_program prog = OK tprog ->
+    forall hf st st' v,
+      Selectionproof.match_states prog tprog hf st st' ->
+      cminor_final_state prog st v ->
+      cminorsel_final_state tprog st' v.
+Proof.
+  intros. invp cminor_final_state.
+  invp Selectionproof.match_states.
+  invp Selectionproof.match_cont.
+  econstructor; eauto.
+  eapply value_inject_swap_ge.
+  instantiate (1 := (Genv.globalenv prog)).
+  eapply value_inject_mem_extends; eauto.
+  intros.
+  unfold Selection.sel_program in *.
+  unfold bind in *.
+  break_match_hyp; try congruence.
+  eapply Selectionproof.function_ptr_translated in H3; eauto.
+  break_exists; break_and. eauto.
+  intros.
+  unfold Selection.sel_program in *.
+  unfold bind in *.
+  break_match_hyp; try congruence.
+  erewrite Selectionproof.symbols_preserved; eauto.
+Qed.
+
+  
+Lemma cminorsel_transf_program_correct :
+  forall (prog : Cminor.program) (tprog : CminorSel.program),
+    Selection.sel_program prog = OK tprog ->
+    forward_simulation (Cminor_semantics prog) (CminorSel_semantics tprog).
+Proof.
+  intros.
+  copy H.
+  unfold Selection.sel_program in H0. unfold bind in *.
+  break_match_hyp; try congruence.
+  eapply forward_simulation_star.
+  eapply Selectionproof.sel_initial_states; eassumption.
+  eapply cminorsel_final_states; eauto.
+  intros.
+  eapply Selectionproof.sel_step_correct in H2; eauto.
+  destruct H2. break_exists. left. eexists. break_and. split.
+  eapply plus_one. eassumption.
+  eauto.
+  right. eauto.
+  eapply Selectionproof.get_helpers_correct; eauto.
+Qed.
